scripts/asm-fixtures/secp256k1FieldSquareFunction.s
@@ -1,0 +1,3 @@
+secf_square_mod_p:
+  mv a1, a0
+  jal zero, secf_mul_mod_p
